theories/bool.ec
@@ -1,0 +1,4 @@
+import why3 "bool" "Bool"
+  op "xorb" as "^^".
+
+op xorb(b0:bool, b1:bool):bool = b0 ^^ b1.
